

Início

Definir

$$f(x, y) = 2x + 2y - x^2 - y^2$$
$$g(x, y) = (x - 2)^2 + y^2 - 2 = 0$$

Calcular os gradientes

$$\nabla f = (2 - 2x, 2 - 2y)$$

$$\nabla g = (2(x - 2), 2y)$$

Montar o sistema de Lagrange

$$\nabla f = \lambda \nabla g$$

$$\Rightarrow \begin{cases} 1 - x = \lambda(x - 2) \\ 1 - y = \lambda y \\ (x - 2)^2 + y^2 = 2 \end{cases}$$

Resolver o sistema

$$\Rightarrow y = 2 - x \text{ e } (x - 2)^2 = 1$$

Pontos candidatos:  $(1, 1)$  e  $(3, -1)$

Avaliar  $f$  nos pontos

$$f(1, 1) = 2, \quad f(3, -1) = -6$$

Classificar

Máximo em  $(1, 1)$  com  $f_{\max} = 2$

Mínimo em  $(3, -1)$  com  $f_{\min} = -6$

Fim